LeanModels/Python/VCTactic.lean
@@ -422,6 +422,7 @@ def interpUnfolds : List Name :=
    ``endsWithUU, ``dunderShaped, ``hasExtraDunder,
    ``findNamedTuple, ``findNamedTupleAux, ``fieldIndex, ``ntupleProtoName,
    ``ntupleMethodName, ``ntupleAttr, ``ntupleCallPlan,
+   ``sliceVal, ``strCallPlan,
    ``RVal.refFree, ``RVal.refFreeList,
    ``Val.listFree, ``Val.listFreeList, ``Val.listFreeArgs,
    ``Heap.get?, ``Heap.update, ``danglingMsg,
